Reorganize material.

lunarlander_sl/ext2/BigStepContinuousEx.thy
@@ -2,13 +2,133 @@ theory BigStepContinuousEx
   imports BigStepContinuous
 begin
 
-subsection \<open>Examples\<close>
-
 definition X :: char where "X = CHR ''x''"
 definition Y :: char where "Y = CHR ''y''"
 definition Z :: char where "Z = CHR ''z''"
 definition ch1 :: cname where "ch1 = ''ch1''"
 definition ch2 :: cname where "ch2 = ''ch2''"
+
+subsection \<open>Basic tests\<close>
+
+lemma test_ode_unique:
+  assumes "spec_of c Q"
+  shows
+  "spec_of (Cont (ODE ((\<lambda>_ _. 0)(X := (\<lambda>_. 1)))) (\<lambda>s. val s X < 1); c)
+           (wait_sol_c (\<lambda>s t. upd s X (val s X + t)) (\<lambda>s. 1 - val s X)
+                       (\<lambda>d s. Q (upd s X (val s X + d))))"
+proof -
+  have 1: "paramODEsol (ODE ((\<lambda>_ _. 0)(X := \<lambda>_. 1))) (\<lambda>s. val s X < 1)
+                       (\<lambda>s t. (rpart s)(X := val s X + t)) (\<lambda>s. 1 - val s X)"
+    unfolding paramODEsol_def apply clarify
+    subgoal for s
+      apply (rule conjI)
+      subgoal apply (cases s)
+        by (auto simp add: rpart.simps val.simps)
+      apply (cases "val s X < 1")
+      subgoal apply auto
+        subgoal
+          unfolding ODEsol_def solves_ode_def has_vderiv_on_def
+          apply auto
+          apply (rule exI[where x="1"])
+          apply auto
+          apply (rule has_vector_derivative_projI)
+          apply (auto simp add: state2vec_def)
+          apply (rule has_vector_derivative_eq_rhs)
+           apply (auto intro!: derivative_intros)[1]
+          by simp
+        subgoal for t
+          apply (cases s) by (auto simp add: updr.simps val.simps)
+        subgoal 
+          apply (cases s) by (auto simp add: updr.simps val.simps)
+        done
+      subgoal by auto
+      done
+    done
+  have 2: "local_lipschitz {- 1<..} UNIV (\<lambda>t v. ODE2Vec (ODE ((\<lambda>_ _. 0)(X := \<lambda>_. 1))) (vec2state v))"
+  proof -
+    have eq: "(\<chi> a. (if a = X then \<lambda>_. 1 else (\<lambda>_. 0)) (($) v)) = (\<chi> a. if a = X then 1 else 0)" for v::vec
+      by auto
+    show ?thesis
+      unfolding fun_upd_def vec2state_def
+      apply (auto simp add: state2vec_def eq)
+      by (rule local_lipschitz_constI)
+  qed
+  show ?thesis
+    apply (rule spec_of_post)
+     apply (rule Valid_cont_unique_sp)
+    apply (rule assms)
+      apply (rule 1) apply (rule 2)
+    apply clarify apply (simp only: updr_rpart_simp1)
+    apply (rule wait_sol_mono) subgoal for _ d' s
+      by (rule entails_triv)
+    done
+qed
+
+lemma test_interrupt_unique:
+  "spec_of (Interrupt (ODE ((\<lambda>_ _. 0)(X := (\<lambda>_. 1)))) (\<lambda>s. val s X < 1)
+                      [(dh[?]Y, Skip)])
+           (interrupt_sol_c (\<lambda>s t. upd s X (val s X + t)) (\<lambda>s. 1 - val s X)
+                            (\<lambda>d s. init (upd s X (val s X + d)))
+                            [InSpec2 dh (\<lambda>d v s. init (upd (upd s X (val s X + d)) Y v))])"
+proof -
+  have 1: "paramODEsol (ODE ((\<lambda>_ _. 0)(X := \<lambda>_. 1))) (\<lambda>s. val s X < 1)
+                       (\<lambda>s0 t. (rpart s0)(X := val s0 X + t)) (\<lambda>s0. 1 - val s0 X)"
+    unfolding paramODEsol_def apply clarify
+    subgoal for s
+      apply (rule conjI)
+      subgoal apply (cases s)
+        by (auto simp add: rpart.simps val.simps)
+      apply (cases "val s X < 1")
+      subgoal apply auto
+        subgoal
+          unfolding ODEsol_def solves_ode_def has_vderiv_on_def
+          apply auto
+          apply (rule exI[where x="1"])
+          apply auto
+          apply (rule has_vector_derivative_projI)
+          apply (auto simp add: state2vec_def)
+          apply (rule has_vector_derivative_eq_rhs)
+           apply (auto intro!: derivative_intros)[1]
+          by simp
+        subgoal for t
+          apply (cases s) by (auto simp add: updr.simps val.simps)
+        subgoal 
+          apply (cases s) by (auto simp add: updr.simps val.simps)
+        done
+      subgoal by auto
+      done
+    done
+  have 2: "local_lipschitz {- 1<..} UNIV (\<lambda>t v. ODE2Vec (ODE ((\<lambda>_ _. 0)(X := \<lambda>_. 1))) (vec2state v))"
+  proof -
+    have eq: "(\<chi> a. (if a = X then \<lambda>_. 1 else (\<lambda>_. 0)) (($) v)) = (\<chi> a. if a = X then 1 else 0)" for v::vec
+      by auto
+    show ?thesis
+      unfolding fun_upd_def vec2state_def
+      apply (auto simp add: state2vec_def eq)
+      by (rule local_lipschitz_constI)
+  qed
+  let ?specs = "[InSpec dh Y init]"
+  show ?thesis
+    apply (rule spec_of_post)
+     apply (rule spec_of_interrupt_unique[where specs="?specs"])
+        apply (rule 1) apply (rule 2)
+      apply auto apply (rule spec_of_es.intros)
+     apply (rule spec_of_skip)
+    subgoal for s0
+      apply (simp only: updr_rpart_simp1)
+      apply (rule interrupt_sol_mono)
+      subgoal by (rule entails_triv)
+      subgoal by auto
+      subgoal for i
+        apply auto apply (intro spec2_entails.intros)
+        subgoal for d v s0 apply (simp only: updr_rpart_simp2)
+          by (rule entails_triv)
+        done
+      done
+    done
+qed
+
+subsection \<open>Examples\<close>
 
 subsubsection \<open>Example 1\<close>
 
@@ -63,7 +183,7 @@ proof -
       apply auto apply (rule spec_of_es.intros)
      apply (rule spec_of_skip)
     subgoal for s0
-      apply (simp only: updr_rpart_simp)
+      apply (simp only: updr_rpart_simp1)
       apply (rule interrupt_solInf_mono)
        apply auto
       apply (intro spec2_entails.intros)
@@ -115,7 +235,7 @@ proof -
       apply auto apply (rule spec_of_es.intros)
      apply (rule spec_of_skip)
     subgoal for s0
-      apply (simp only: updr_rpart_simp)
+      apply (simp only: updr_rpart_simp1)
       apply (rule interrupt_solInf_mono)
        apply auto
       apply (intro spec2_entails.intros)
@@ -160,485 +280,6 @@ lemma ex1b_sp:
    apply (rule Valid_wait_sp)
    apply (rule spec_of_send)
   apply auto by (rule entails_triv)
-
-datatype 'a comm_specg2 =
-  InSpecg2 cname "real \<Rightarrow> real \<Rightarrow> 'a gassn2"
-| OutSpecg2 cname "real \<Rightarrow> 'a gstate \<Rightarrow> real" "real \<Rightarrow> 'a gassn2"
-
-text \<open>Mapping from path on a single state to path on general states\<close>
-definition single_path :: "pname \<Rightarrow> ('a estate \<Rightarrow> real \<Rightarrow> 'a estate) \<Rightarrow> 'a gstate \<Rightarrow> real \<Rightarrow> 'a gstate" where
-  "single_path pn p gs t = gs (pn \<mapsto> p (the (gs pn)) t)"
-
-lemma single_path_State:
-  "single_path pn p (State pn s) t = State pn (p s t)"
-  unfolding single_path_def
-  by (auto simp add: State_def)
-
-text \<open>Merging two paths\<close>
-definition restrict_state :: "pname set \<Rightarrow> 'a gstate \<Rightarrow> 'a gstate" where
-  "restrict_state pns gs = (\<lambda>pn. if pn \<in> pns then gs pn else None)"
-
-definition merge_path :: "pname set \<Rightarrow> pname set \<Rightarrow>
-                          ('a gstate \<Rightarrow> real \<Rightarrow> 'a gstate) \<Rightarrow> ('a gstate \<Rightarrow> real \<Rightarrow> 'a gstate) \<Rightarrow>
-                          ('a gstate \<Rightarrow> real \<Rightarrow> 'a gstate)" where
-  "merge_path pns1 pns2 p1 p2 = (\<lambda>gs t.
-     merge_state (p1 (restrict_state pns1 gs) t) (p2 (restrict_state pns2 gs) t))"
-
-fun delay_path :: "real \<Rightarrow> ('a gstate \<Rightarrow> real \<Rightarrow> 'a gstate) \<Rightarrow> ('a gstate \<Rightarrow> real \<Rightarrow> 'a gstate)" where
-  "delay_path d p gs d' = p gs (d' + d)"
-
-lemma restrict_state_eval1:
-  assumes "proc_set gs1 = pns1"
-  shows "restrict_state pns1 (merge_state gs1 gs2) = gs1"
-  apply (rule ext) subgoal for pn
-    unfolding restrict_state_def apply auto
-     apply (subst merge_state_eval1) using assms apply auto
-    unfolding proc_set_def by auto
-  done
-
-lemma restrict_state_eval2:
-  assumes "proc_set gs1 = pns1"
-    and "proc_set gs2 = pns2"
-    and "pns1 \<inter> pns2 = {}"
-  shows "restrict_state pns2 (merge_state gs1 gs2) = gs2"
-  apply (rule ext) subgoal for pn
-    unfolding restrict_state_def apply auto
-     apply (subst merge_state_eval2) using assms apply auto
-    unfolding proc_set_def by auto
-  done
-
-lemma merge_path_eval:
-  assumes "proc_set gs1 = pns1"
-    and "proc_set gs2 = pns2"
-    and "pns1 \<inter> pns2 = {}"
-  shows
-  "merge_path pns1 pns2 p1 p2 (merge_state gs1 gs2) t = merge_state (p1 gs1 t) (p2 gs2 t)"
-  unfolding merge_path_def
-  by (auto simp add: restrict_state_eval1 restrict_state_eval2 assms)
-
-fun id_path :: "'a gstate \<Rightarrow> real \<Rightarrow> 'a gstate" where
-  "id_path gs t = gs"
-
-fun single_val :: "pname \<Rightarrow> 'a eexp \<Rightarrow> 'a gstate \<Rightarrow> real" where
-  "single_val pn e gs = e (the (gs pn))"
-
-text \<open>Mapping from specification on single state to specification
-  on general states.
-\<close>
-fun gassn_of :: "pname \<Rightarrow> 'a comm_spec2 \<Rightarrow> 'a comm_specg2" where
-  "gassn_of pn (InSpec2 ch Q) = InSpecg2 ch (\<lambda>d v. single_assn pn (Q d v))"
-| "gassn_of pn (OutSpec2 ch e Q) = OutSpecg2 ch (\<lambda>d. single_val pn (e d)) (\<lambda>d. single_assn pn (Q d))"
-
-fun rdy_of_comm_specg2 :: "'a comm_specg2 list \<Rightarrow> rdy_info" where
-  "rdy_of_comm_specg2 [] = ({}, {})"
-| "rdy_of_comm_specg2 (InSpecg2 ch P # rest) = (
-    let rdy = rdy_of_comm_specg2 rest in
-      (insert ch (fst rdy), snd rdy))"
-| "rdy_of_comm_specg2 (OutSpecg2 ch e P # rest) = (
-    let rdy = rdy_of_comm_specg2 rest in
-      (fst rdy, insert ch (snd rdy)))"
-
-lemma rdy_of_comm_spec_gassn_of:
-  "rdy_of_comm_spec2 specs = rdy_of_comm_specg2 (map (gassn_of pn) specs)"
-  sorry
-
-inductive interrupt_solInf_cg :: "('a gstate \<Rightarrow> real \<Rightarrow> 'a gstate) \<Rightarrow> 'a comm_specg2 list \<Rightarrow> 'a gassn2" where
-  "i < length specs \<Longrightarrow> specs ! i = InSpecg2 ch Q \<Longrightarrow>
-   Q 0 v gs0 gs tr \<Longrightarrow> interrupt_solInf_cg p specs gs0 gs (InBlockP ch v # tr)"
-| "i < length specs \<Longrightarrow> specs ! i = InSpecg2 ch Q \<Longrightarrow>
-   0 < d \<Longrightarrow> Q d v gs0 gs tr \<Longrightarrow> p' = (\<lambda>\<tau>\<in>{0..d}. p gs0 \<tau>) \<Longrightarrow>
-   rdy = rdy_of_comm_specg2 specs \<Longrightarrow>
-   interrupt_solInf_cg p specs gs0 gs (WaitBlockP d p' rdy # InBlockP ch v # tr)"
-| "i < length specs \<Longrightarrow> specs ! i = OutSpecg2 ch e Q \<Longrightarrow>
-   v = e 0 gs0 \<Longrightarrow>
-   Q 0 gs0 gs tr \<Longrightarrow> interrupt_solInf_cg p specs gs0 gs (OutBlockP ch v # tr)"
-| "i < length specs \<Longrightarrow> specs ! i = OutSpecg2 ch e Q \<Longrightarrow>
-   0 < d \<Longrightarrow> Q d gs0 gs tr \<Longrightarrow> p' = (\<lambda>\<tau>\<in>{0..d}. p gs0 \<tau>) \<Longrightarrow>
-   v = e d gs0 \<Longrightarrow>
-   rdy = rdy_of_comm_specg2 specs \<Longrightarrow>
-   interrupt_solInf_cg p specs gs0 gs (WaitBlockP d p' rdy # OutBlockP ch v # tr)"
-
-lemma single_assn_interrupt_solInf:
-  "single_assn pn (interrupt_solInf_c p specs) =
-   interrupt_solInf_cg (single_path pn p) (map (gassn_of pn) specs)"
-  apply (rule ext) apply (rule ext) apply (rule ext)
-  subgoal for s0 s tr
-    apply (rule iffI)
-    subgoal apply (elim single_assn.cases) apply auto
-      subgoal for s0' s' tr'
-        apply (elim interrupt_solInf_c.cases) apply auto
-        subgoal for i ch Q v tr''
-          apply (rule interrupt_solInf_cg.intros(1)[of i _ _ "(\<lambda>d v. single_assn pn (Q d v))"])
-          by (auto intro: single_assn.intros)
-        subgoal premises pre for i ch Q d v tr'' a b
-          apply (rule interrupt_solInf_cg.intros(2)[of i _ _ "(\<lambda>d v. single_assn pn (Q d v))"])
-          unfolding single_path_State
-          using pre rdy_of_comm_spec_gassn_of by (auto intro: single_assn.intros)
-        subgoal for i ch e Q tr''
-          apply (rule interrupt_solInf_cg.intros(3)[of i _ _ "(\<lambda>d. single_val pn (e d))" "(\<lambda>d. single_assn pn (Q d))" ])
-          by (auto intro: single_assn.intros)
-        subgoal premises pre for i ch e Q d tr'' a b
-          apply (rule interrupt_solInf_cg.intros(4)[of i _ _ "(\<lambda>d. single_val pn (e d))" "(\<lambda>d. single_assn pn (Q d))"])
-          unfolding single_path_State
-          using pre rdy_of_comm_spec_gassn_of by (auto intro: single_assn.intros)
-        done
-      done
-    subgoal apply (elim interrupt_solInf_cg.cases) apply auto
-      subgoal for i ch Q v tr'
-        apply (cases "specs ! i") apply auto
-        apply (elim single_assn.cases) apply auto
-        subgoal for Q' s0' s' tr''
-          apply (subst ptrace_of.simps[symmetric])
-          apply (rule single_assn.intros)
-          apply (rule interrupt_solInf_c.intros(1)[of i _ _ Q']) by auto
-        done
-      subgoal for i ch Q d v tr' a b
-        apply (cases "specs ! i") apply auto
-        apply (elim single_assn.cases) apply auto
-        subgoal for Q' s0'' s' tr''
-          unfolding single_path_State
-          apply (subst ptrace_of.simps(2)[symmetric])
-          apply (subst ptrace_of_simp3[symmetric])
-          apply (rule single_assn.intros)
-          apply (rule interrupt_solInf_c.intros(2)[of i _ _ Q']) apply auto
-          unfolding rdy_of_comm_spec_gassn_of[symmetric] by auto
-        done
-      subgoal for i ch e Q tr'
-        apply (cases "specs ! i") apply auto
-        apply (elim single_assn.cases) apply auto
-        subgoal for e' Q' s0'' s' tr''
-          apply (subst ptrace_of.simps[symmetric])
-          apply (rule single_assn.intros)
-          apply (rule interrupt_solInf_c.intros(3)[of i _ _ _ Q']) by auto
-        done
-      subgoal for i ch e Q d tr' a b
-        apply (cases "specs ! i") apply auto
-        apply (elim single_assn.cases) apply auto
-        subgoal for e' Q' s0'' s' tr''
-          unfolding single_path_State
-          apply (subst ptrace_of.simps[symmetric])
-          apply (subst ptrace_of_simp3[symmetric])
-          apply (rule single_assn.intros)
-          apply (rule interrupt_solInf_c.intros(4)[of i _ _ _ Q']) apply auto
-          unfolding rdy_of_comm_spec_gassn_of[symmetric] by auto
-        done
-      done
-    done
-  done
-
-definition disj_gassn :: "'a gassn2 \<Rightarrow> 'a gassn2 \<Rightarrow> 'a gassn2" (infixr "\<or>\<^sub>g" 35) where
-  "(P \<or>\<^sub>g Q) gs0 = (\<lambda>gs tr. P gs0 gs tr \<or> Q gs0 gs tr)"
-
-lemma single_assn_disj:
-  "single_assn pn (P \<or>\<^sub>a Q) = (single_assn pn P \<or>\<^sub>g single_assn pn Q)"
-  apply (rule ext) apply (rule ext) apply (rule ext)
-  subgoal for s0 s tr
-    apply (rule iffI)
-    subgoal apply (elim single_assn.cases) apply auto
-      subgoal for s0' s' tr'
-        unfolding disj_gassn_def disj_assn2_def
-        by (auto intro: single_assn.intros)
-      done
-    subgoal unfolding disj_gassn_def disj_assn2_def
-      apply (elim disjE single_assn.cases)
-      by (auto intro: single_assn.intros)
-    done
-  done
-
-lemma sync_gassn_disj:
-  assumes "sync_gassn chs pns1 pns2 P1 Q gs0 \<Longrightarrow>\<^sub>g R"
-    and "sync_gassn chs pns1 pns2 P2 Q gs0 \<Longrightarrow>\<^sub>g R"
-  shows "sync_gassn chs pns1 pns2 (P1 \<or>\<^sub>g P2) Q gs0 \<Longrightarrow>\<^sub>g R"
-  unfolding entails_g_def apply auto
-  subgoal for s tr
-    apply (elim sync_gassn.cases) apply auto
-    using assms unfolding disj_gassn_def entails_g_def
-    by (auto simp add: sync_gassn.intros)
-  done
-
-lemma sync_gassn_disj2:
-  assumes "sync_gassn chs pns1 pns2 P1 Q gs0 \<Longrightarrow>\<^sub>g R1 gs1"
-    and "sync_gassn chs pns1 pns2 P2 Q gs0 \<Longrightarrow>\<^sub>g R2 gs1"
-  shows "sync_gassn chs pns1 pns2 (P1 \<or>\<^sub>g P2) Q gs0 \<Longrightarrow>\<^sub>g (R1 \<or>\<^sub>g R2) gs1"
-  unfolding entails_g_def apply auto
-  subgoal for s tr
-    apply (elim sync_gassn.cases) apply auto
-    using assms unfolding disj_gassn_def entails_g_def
-    by (auto simp add: sync_gassn.intros)
-  done
-
-lemma entails_g_disj:
-  assumes "P1 gs0 \<Longrightarrow>\<^sub>g R gs0"
-    and "P2 gs0 \<Longrightarrow>\<^sub>g R gs0"
-  shows "(P1 \<or>\<^sub>g P2) gs0 \<Longrightarrow>\<^sub>g R gs0"
-  using assms unfolding entails_g_def disj_gassn_def by auto
-
-lemma entails_g_disj2:
-  assumes "P1 gs0 \<Longrightarrow>\<^sub>g R1 gs0"
-    and "P2 gs0 \<Longrightarrow>\<^sub>g R2 gs0"
-  shows "(P1 \<or>\<^sub>g P2) gs0 \<Longrightarrow>\<^sub>g (R1 \<or>\<^sub>g R2) gs0"
-  using assms unfolding entails_g_def disj_gassn_def by auto
-
-fun spec_wait_of :: "real \<Rightarrow> ('a gstate \<Rightarrow> real \<Rightarrow> 'a gstate) \<Rightarrow> 'a comm_specg2 \<Rightarrow> 'a comm_specg2" where
-  "spec_wait_of d p (InSpecg2 ch P) = InSpecg2 ch (\<lambda>d' v. P (d + d') v)"
-| "spec_wait_of d p (OutSpecg2 ch e P) = OutSpecg2 ch (\<lambda>d' gs. e (d + d') gs) (\<lambda>d'. P (d + d'))"
-
-inductive wait_sol_cg :: "('a gstate \<Rightarrow> real \<Rightarrow> 'a gstate) \<Rightarrow> pname \<Rightarrow> 'a eexp \<Rightarrow>
-                          (real \<Rightarrow> 'a gassn2) \<Rightarrow> 'a gassn2" where
-  "e (the (gs0 pn)) > 0 \<Longrightarrow> d = e (the (gs0 pn)) \<Longrightarrow> p' = (\<lambda>t\<in>{0..d}. p gs0 t) \<Longrightarrow>
-   P d gs0 gs tr \<Longrightarrow> rdy = ({}, {}) \<Longrightarrow>
-   wait_sol_cg p pn e P gs0 gs (WaitBlockP d p' rdy # tr)"
-| "\<not>e (the (gs0 pn)) > 0 \<Longrightarrow> P 0 gs0 gs tr \<Longrightarrow> wait_sol_cg p pn e P gs0 gs tr"
-
-lemma wait_sol_cg_mono:
-  assumes "\<And>d s0. P1 d s0 \<Longrightarrow>\<^sub>g P2 d s0"
-  shows "wait_sol_cg p pn e P1 s0 \<Longrightarrow>\<^sub>g wait_sol_cg p pn e P2 s0"
-  apply (auto simp add: entails_g_def)
-  subgoal for s tr
-    apply (elim wait_sol_cg.cases) apply auto
-    subgoal apply (rule wait_sol_cg.intros)
-      using assms unfolding entails_g_def by auto
-    subgoal apply (rule wait_sol_cg.intros)
-      using assms unfolding entails_g_def by auto
-    done
-  done
-
-lemma compat_rdy_empty [simp]:
-  "compat_rdy rdy ({}, {})"
-  apply (cases rdy) by auto
-
-fun ch_of_specg2 :: "'a comm_specg2 \<Rightarrow> cname" where
-  "ch_of_specg2 (InSpecg2 ch P) = ch"
-| "ch_of_specg2 (OutSpecg2 ch e P) = ch"
-
-lemma merge_rdy_simp1:
-  assumes "\<And>i. i < length specs \<Longrightarrow> ch_of_specg2 (specs ! i) \<in> chs"
-  shows "merge_rdy chs (rdy_of_comm_specg2 specs) ({}, {}) = ({}, {})"
-  sorry
-
-lemma rdy_of_spec_wait_of [simp]:
-  "rdy_of_comm_specg2 (map (spec_wait_of d p) specs) = rdy_of_comm_specg2 specs"
-  sorry
-
-lemma sync_gassn_interrupt_solInf_wait:
-  assumes "pn2 \<in> pns2"
-    and "pns1 \<inter> pns2 = {}"
-    and "\<And>i. i < length specs \<Longrightarrow> ch_of_specg2 (specs ! i) \<in> chs"
-  shows
-  "sync_gassn chs pns1 pns2 (interrupt_solInf_cg p specs) (wait_cg pn2 e Q) s0 \<Longrightarrow>\<^sub>g
-   wait_sol_cg (merge_path pns1 pns2 p id_path) pn2 e
-    (\<lambda>d. sync_gassn chs pns1 pns2 (interrupt_solInf_cg (delay_path d p) (map (spec_wait_of d p) specs)) Q) s0"
-  unfolding entails_g_def apply auto
-  subgoal for s tr
-    apply (elim sync_gassn.cases) apply auto
-    subgoal for s11 s12 s21 s22 tr1 tr2
-      apply (elim interrupt_solInf_cg.cases) apply auto
-      subgoal for i ch Q' v tr'
-        apply (elim wait_cg.cases) apply auto
-        subgoal for tr''
-          apply (elim combine_blocks_pairE2)
-          using assms(3)[of i] by auto
-        subgoal
-          apply (rule wait_sol_cg.intros(2))
-          apply (subst merge_state_eval2)
-          using assms apply auto
-          apply (rule sync_gassn.intros) apply auto
-          apply (rule interrupt_solInf_cg.intros(1)[of i _ _ Q'])
-          by auto
-        done
-      subgoal for i ch Q' d' v tr' a b
-        apply (elim wait_cg.cases) apply auto
-        subgoal for tr''
-          apply (cases rule: linorder_cases[of d' "e (the (s12 pn2))"])
-          subgoal
-            apply (elim combine_blocks_waitE3) apply auto
-            apply (elim combine_blocks_pairE2)
-            using assms(3)[of i] by auto
-          subgoal apply auto
-            apply (elim combine_blocks_waitE2) apply auto
-            subgoal for tr'''
-              apply (rule wait_sol_cg.intros(1))
-              subgoal apply (subst merge_state_eval2)
-                using assms(1,2) by auto
-              subgoal apply (subst merge_state_eval2)
-                using assms(1,2) by auto
-              subgoal apply (rule ext) apply auto
-                apply (subst merge_path_eval)
-                using assms by auto
-              apply (rule sync_gassn.intros) apply auto
-              apply (rule interrupt_solInf_cg.intros(1)[of i _ _ "\<lambda>d' v. Q' (e (the (s12 pn2)) + d') v"])
-              apply auto apply (rule merge_rdy_simp1) using assms(3) by auto
-            done
-          subgoal
-            apply (elim combine_blocks_waitE4) apply auto
-            subgoal for tr'''
-              apply (rule wait_sol_cg.intros(1))
-              subgoal apply (subst merge_state_eval2)
-                using assms(1,2) by auto
-              subgoal apply (subst merge_state_eval2)
-                using assms(1,2) by auto
-              subgoal apply (rule ext) apply auto
-                apply (subst merge_path_eval)
-                using assms by auto
-              apply (rule sync_gassn.intros) apply auto
-              apply (rule interrupt_solInf_cg.intros(2)[of i _ _ "\<lambda>d' v. Q' (e (the (s12 pn2)) + d') v"])
-              apply auto apply (rule merge_rdy_simp1) using assms(3) by auto
-            done
-          done
-        subgoal
-          apply (rule wait_sol_cg.intros(2))
-          subgoal apply (subst merge_state_eval2)
-            using assms(1,2) by auto
-          apply (rule sync_gassn.intros) apply auto
-          apply (rule interrupt_solInf_cg.intros(2)[of i _ _ Q'])
-          by auto
-        done
-      subgoal for i ch e Q' tr'
-        apply (elim wait_cg.cases) apply auto
-        subgoal for tr''
-          apply (elim combine_blocks_pairE2)
-          using assms(3)[of i] by auto
-        subgoal
-          apply (rule wait_sol_cg.intros(2))
-          apply (subst merge_state_eval2)
-          using assms apply auto
-          apply (rule sync_gassn.intros) apply auto
-          apply (rule interrupt_solInf_cg.intros(3)[of i _ _ e Q'])
-          by auto
-        done
-      subgoal for i ch e' Q' d' tr' a b
-        apply (elim wait_cg.cases) apply auto
-        subgoal for tr''
-          apply (cases rule: linorder_cases[of d' "e (the (s12 pn2))"])
-          subgoal
-            apply (elim combine_blocks_waitE3) apply auto
-            apply (elim combine_blocks_pairE2)
-            using assms(3)[of i] by auto
-          subgoal apply auto
-            apply (elim combine_blocks_waitE2) apply auto
-            subgoal for tr'''
-              apply (rule wait_sol_cg.intros(1))
-              subgoal apply (subst merge_state_eval2)
-                using assms(1,2) by auto
-              subgoal apply (subst merge_state_eval2)
-                using assms(1,2) by auto
-              subgoal apply (rule ext) apply auto
-                apply (subst merge_path_eval)
-                using assms by auto
-              apply (rule sync_gassn.intros) apply auto
-              apply (rule interrupt_solInf_cg.intros(3)[of i _ _ "\<lambda>d'. e' (e (the (s12 pn2)) + d')"
-                                                                 "\<lambda>d'. Q' (e (the (s12 pn2)) + d')"])
-              apply auto apply (rule merge_rdy_simp1) using assms(3) by auto
-            done
-          subgoal
-            apply (elim combine_blocks_waitE4) apply auto
-            subgoal for tr'''
-              apply (rule wait_sol_cg.intros(1))
-              subgoal apply (subst merge_state_eval2)
-                using assms(1,2) by auto
-              subgoal apply (subst merge_state_eval2)
-                using assms(1,2) by auto
-              subgoal apply (rule ext) apply auto
-                apply (subst merge_path_eval)
-                using assms by auto
-              apply (rule sync_gassn.intros) apply auto
-              apply (rule interrupt_solInf_cg.intros(4)[of i _ _ "\<lambda>d'. e' (e (the (s12 pn2)) + d')"
-                                                                 "\<lambda>d' v. Q' (e (the (s12 pn2)) + d') v"])
-              apply auto apply (rule merge_rdy_simp1) using assms(3) by auto
-            done
-          done
-        subgoal
-          apply (rule wait_sol_cg.intros(2))
-          subgoal apply (subst merge_state_eval2)
-            using assms(1,2) by auto
-          apply (rule sync_gassn.intros) apply auto
-          apply (rule interrupt_solInf_cg.intros(4)[of i _ _ e' Q'])
-          by auto
-        done
-      done
-    done
-  done
-
-lemma not_compat_rdy_comm_specg2:
-  assumes "i < length specs"
-    and "specs ! i = InSpecg2 ch P"
-  shows
-    "\<not> compat_rdy (rdy_of_comm_specg2 specs) ({ch}, {})"
-  sorry
-
-text \<open>Synchronization between interrupt and synchronized output
-  Assume there is a corresponding input in the interrupt. Then
-  the communication happens immediately.
-\<close>
-lemma sync_gassn_interrupt_solInf_out:
-  assumes "pn2 \<in> pns2"
-    and "pns1 \<inter> pns2 = {}"
-    and "\<And>i. i < length specs \<Longrightarrow> ch_of_specg2 (specs ! i) \<in> chs"
-    and "\<And>i j. i < length specs \<Longrightarrow> j < length specs \<Longrightarrow> i \<noteq> j \<Longrightarrow>
-               ch_of_specg2 (specs ! i) \<noteq> ch_of_specg2 (specs ! j)"
-    and "i < length specs"
-    and "specs ! i = InSpecg2 ch P"
-  shows
-  "sync_gassn chs pns1 pns2 (interrupt_solInf_cg p specs)
-                            (wait_out_cg pn2 ch e Q) s0 \<Longrightarrow>\<^sub>g
-   sync_gassn chs pns1 pns2 (P 0 (e (the (s0 pn2)))) (Q 0) s0"
-  unfolding entails_g_def apply auto
-  subgoal for s tr
-    apply (elim sync_gassn.cases) apply auto
-    subgoal for s11 s12 s21 s22 tr1 tr2
-      apply (elim interrupt_solInf_cg.cases) apply auto
-      subgoal for i' ch' Q' v tr'
-        apply (elim wait_out_cg.cases) apply auto
-        subgoal for tr''
-          apply (cases "i = i'")
-          subgoal using assms(5,6) apply auto
-            apply (elim combine_blocks_pairE)
-            using assms(3) apply fastforce
-            using assms(3) apply fastforce
-            apply (rule sync_gassn.intros)
-            using assms by (auto simp add: assms merge_state_eval2)
-          subgoal
-            apply (elim combine_blocks_pairE)
-            using assms(3) apply fastforce
-            apply (metis assms(3,5,6) ch_of_specg2.simps(1))
-            by (metis assms(4,5,6) ch_of_specg2.simps(1))
-          done
-        subgoal for d tr''
-          apply (elim combine_blocks_pairE2)
-          using assms(3) by fastforce
-        done
-      subgoal for i ch' Q' d v tr' a b
-        apply (elim wait_out_cg.cases) apply auto
-        subgoal for tr''
-          apply (elim combine_blocks_pairE2')
-          by (metis assms(3,5,6) ch_of_specg2.simps(1))
-        subgoal for d' tr''
-          apply (elim combine_blocks_waitE1)
-          apply (rule not_compat_rdy_comm_specg2) using assms(5,6) by auto
-        done
-      subgoal for i ch' e' Q' tr'
-        apply (elim wait_out_cg.cases) apply auto
-        subgoal for tr''
-          apply (elim combine_blocks_pairE)
-          using assms(3) apply fastforce
-           apply (metis assms(3,5,6) ch_of_specg2.simps(1))
-          by auto
-        subgoal for d' tr''
-          apply (elim combine_blocks_pairE2)
-          using assms(3) by fastforce
-        done
-      subgoal for i ch' e' Q' d tr' a b
-        apply (elim wait_out_cg.cases) apply auto
-        subgoal for tr''
-          apply (elim combine_blocks_pairE2')
-          by (metis assms(3,5,6) ch_of_specg2.simps(1))
-        subgoal for d' tr''
-          apply (elim combine_blocks_waitE1)
-          apply (rule not_compat_rdy_comm_specg2) using assms(5,6) by auto
-        done
-      done
-    done
-  done
 
 lemma ex1':
   "spec_of_global
@@ -716,110 +357,29 @@ lemma ex1':
     done
   done
 
-
-text \<open>Basic assertion for invariants: wait for the specified amount of time,
-  while all states in the path satisfy the given invariant, then the remaining
-  trace satisfy the following assertion.
-\<close>
-inductive wait_inv_cg :: "('a gstate \<Rightarrow> bool) \<Rightarrow> 'a gassn2 \<Rightarrow> 'a gassn2" where
-  "d > 0 \<Longrightarrow> rdy = ({}, {}) \<Longrightarrow> \<forall>t\<in>{0..d}. I (p t) \<Longrightarrow> P gs0 gs tr \<Longrightarrow>
-   wait_inv_cg I P gs0 gs (WaitBlockP d (\<lambda>t\<in>{0..d}. p t) rdy # tr)"
-
-lemma wait_inv_cg_state:
-  "wait_inv_cg I P (updg s0 pn var x) \<Longrightarrow>\<^sub>g wait_inv_cg I (\<lambda>s. P (updg s pn var x)) s0"
-  unfolding entails_g_def apply auto
-  subgoal for s tr
-    apply (elim wait_inv_cg.cases) apply auto
-    subgoal for p tr'
-      apply (rule wait_inv_cg.intros) by auto
-    done
-  done
-
-lemma wait_inv_cgI:
-  assumes "e (the (gs0 pn)) = d"
-    and "d > 0"
-    and "\<forall>t\<in>{0..d}. I (p gs0 t)"
-  shows "wait_sol_cg p pn e P gs0 \<Longrightarrow>\<^sub>g wait_inv_cg I (P d) gs0"
-  unfolding entails_g_def apply auto
-  subgoal for s tr
-    apply (elim wait_sol_cg.cases) apply auto
-    using assms by (auto intro: wait_inv_cg.intros)
-  done
-
-lemma wait_inv_cg_mono:
-  assumes "P1 s0 \<Longrightarrow>\<^sub>g P2 s0"
-  shows "wait_inv_cg I P1 s0 \<Longrightarrow>\<^sub>g wait_inv_cg I P2 s0"
-  unfolding entails_g_def apply auto
-  subgoal for s tr
-    apply (elim wait_inv_cg.cases) apply auto
-    apply (rule wait_inv_cg.intros) apply auto
-    using assms unfolding entails_g_def by auto
-  done
-
-lemma merge_restrict:
-  assumes "proc_set s = pns1 \<union> pns2"
-    and "pns1 \<inter> pns2 = {}"
-  shows "merge_state (restrict_state pns1 s) (restrict_state pns2 s) = s"
-  unfolding merge_state_def restrict_state_def
-  apply (rule ext) apply auto
-  using assms(1,2) unfolding proc_set_def apply auto
-  subgoal for p apply (cases "s p") by auto
-  subgoal for p apply (cases "s p") by auto
-  done
-
-lemma proc_set_restrict_state:
-  assumes "pns1 \<subseteq> proc_set s"
-  shows "proc_set (restrict_state pns1 s) = pns1"
-  using assms unfolding restrict_state_def proc_set_def by auto
-
-lemma merge_state_elim:
-  assumes "proc_set s = pns1 \<union> pns2"
-    and "pns1 \<inter> pns2 = {}"
-    and "\<And>s1 s2. s = merge_state s1 s2 \<Longrightarrow> proc_set s1 = pns1 \<Longrightarrow> proc_set s2 = pns2 \<Longrightarrow> P"
-  shows P
-  apply (rule assms(3)[of "restrict_state pns1 s" "restrict_state pns2 s"])
-  by (auto simp add: merge_restrict proc_set_restrict_state assms)  
-
-lemma merge_state_updg_left:
-  assumes "pn \<in> proc_set s1"
-  shows "merge_state (updg s1 pn v e) s2 = updg (merge_state s1 s2) pn v e"
-  apply (rule ext)
-  using assms by (auto simp add: proc_set_def merge_state_def updg_def)
-
-lemma valg_merge_state_left:
-  assumes "pn \<in> proc_set s1"
-  shows "valg (merge_state s1 s2) pn v = valg s1 pn v"
-  using assms by (auto simp add: proc_set_def merge_state_def valg_def)
-
-lemma merge_test:
+lemma ex1_merge1:
   assumes "proc_set s0 = {''a'', ''b''}"
   shows
   "merge_path {''a''} {''b''} (single_path ''a'' (\<lambda>s t. upd s X (val s X + 2 * t))) id_path s0 =
    (\<lambda>t. updg s0 ''a'' X (valg s0 ''a'' X + 2 * t))"
   apply (rule merge_state_elim[of s0 "{''a''}" "{''b''}"])
-  using assms apply auto[1] apply auto[1]
-  subgoal for s1 s2
-    apply simp apply (rule ext) subgoal for t
-      apply (subst merge_path_eval) apply auto[1] apply auto[1] apply auto[1]
-      by (simp add: single_path_def valg_def[symmetric] updg_def[symmetric]
-                    merge_state_updg_left valg_merge_state_left)
-    done
-  done
+  using assms apply auto[2]
+  apply simp apply (rule ext)
+  apply (subst merge_path_eval) apply auto[3]
+  by (simp add: single_path_def valg_def[symmetric] updg_def[symmetric]
+      merge_state_updg_left valg_merge_state_left)
 
-lemma merge_test2:
+lemma ex1_merge2:
   assumes "proc_set s0 = {''a'', ''b''}"
   shows
   "merge_path {''a''} {''b''} (single_path ''a'' (\<lambda>s t. upd s X (val s X + t))) id_path s0 =
    (\<lambda>t. updg s0 ''a'' X (valg s0 ''a'' X + t))"
   apply (rule merge_state_elim[of s0 "{''a''}" "{''b''}"])
-  using assms apply auto[1] apply auto[1]
-  subgoal for s1 s2
-    apply simp apply (rule ext) subgoal for t
-      apply (subst merge_path_eval) apply auto[1] apply auto[1] apply auto[1]
-      by (simp add: single_path_def valg_def[symmetric] updg_def[symmetric]
-                    merge_state_updg_left valg_merge_state_left)
-    done
-  done
+  using assms apply auto[2]
+  apply simp apply (rule ext)
+  apply (subst merge_path_eval) apply auto[3]
+  by (simp add: single_path_def valg_def[symmetric] updg_def[symmetric]
+      merge_state_updg_left valg_merge_state_left)
 
 lemma ex1'':
   assumes "proc_set s0 = {''a'', ''b''}"
@@ -849,7 +409,7 @@ lemma ex1'':
      apply (rule wait_inv_cgI[where d=1 and I="\<lambda>gs. valg gs ''a'' X \<in> {0..2}"])
        apply (simp only: valg_def[symmetric]) apply auto[1]
       apply auto[1]
-    subgoal apply (subst merge_test)
+    subgoal apply (subst ex1_merge1)
       using assms by auto
     apply (rule entails_g_trans)
      apply (rule wait_inv_cg_state)
@@ -874,7 +434,7 @@ lemma ex1'':
      apply (rule wait_inv_cgI[where d=2 and I="\<lambda>gs. valg gs ''a'' X \<in> {0..2}"])
        apply (simp only: valg_def[symmetric]) apply auto[1]
       apply auto[1]
-    subgoal apply (subst merge_test2)
+    subgoal apply (subst ex1_merge2)
       using assms by auto
     apply (rule entails_g_trans)
      apply (rule wait_inv_cg_state)
